SystemFD/Metatheory/FrameWf.lean
@@ -1,0 +1,220 @@
+import SystemFD.Term
+import SystemFD.Judgment
+import SystemFD.Ctx
+import SystemFD.Metatheory.Weaken
+import SystemFD.Metatheory.TypeMatch
+
+namespace FrameWf
+  theorem weaken (r : Ren) :
+    ⊢ Δ ->
+    (∀ x, (Γ d@ x).apply r.to = Δ d@ (r x)) ->
+    Γ ⊢ f -> Δ ⊢ f.apply r.to
+  := by
+  intro wf h j
+  cases j
+  case _ =>
+    unfold Frame.apply; simp; constructor
+    apply wf
+  case _ j =>
+    unfold Frame.apply; simp; constructor
+    have lem := rename r j wf h; simp at lem
+    apply lem
+  case _ j =>
+    unfold Frame.apply; simp; constructor
+    have lem := rename r j wf h; simp at lem
+    apply lem
+  case _ j =>
+    unfold Frame.apply; simp; constructor
+    have lem := rename r j wf h; simp at lem
+    apply lem
+  case _ j1 j2 =>
+    unfold Frame.apply; simp; constructor
+    have lem := rename r j1 wf h; simp at lem
+    apply lem; apply valid_ctor_subst _ _ j2
+    case _ =>
+      intro n y h2; rw [h]
+      unfold Ren.to at h2; simp at h2; subst h2
+      simp
+    case _ =>
+      intro n h2; unfold Ren.to; simp
+  case _ j =>
+    unfold Frame.apply; simp; constructor
+    have lem := rename r j wf h; simp at lem
+    apply lem
+  case _ j =>
+    unfold Frame.apply; simp; constructor
+    have lem := rename r j wf h; simp at lem
+    apply lem
+  case _ j1 j2 =>
+    unfold Frame.apply; simp; constructor
+    have lem := rename r j1 wf h; simp at lem
+    apply lem; apply valid_insttype_subst _ _ j2
+    case _ =>
+      intro n y h2; rw [h]
+      unfold Ren.to at h2; simp at h2; subst h2
+      simp
+    case _ =>
+      intro n h2; unfold Ren.to; simp
+  case _ x T t j1 j2 =>
+    have h2 := h x; rw [<-j1] at h2
+    unfold Frame.apply at h2; simp at h2
+    constructor; apply h2
+    have lem := rename r j2 wf h; simp at lem
+    apply lem
+  case _ j1 j2 =>
+    unfold Frame.apply; simp; constructor
+    have lem1 := rename r j1 wf h; simp at lem1; apply lem1
+    have lem2 := rename r j2 wf h; simp at lem2; apply lem2
+end FrameWf
+
+@[simp]
+abbrev FrameWfByIndexLemmaType (Γ : Ctx Term) : (v : JudgmentVariant) -> JudgmentArgs v -> Prop
+| .prf => λ _ => True
+| .wf => λ () => ∀ x, Γ ⊢ Γ d@ x
+
+theorem frame_wf_by_index_lemma : Judgment v Γ ix -> FrameWfByIndexLemmaType Γ v ix := by
+intro j; induction j <;> simp at *
+case _ => constructor; constructor
+case _ wf ih =>
+  intro x; cases x <;> simp at *
+  case _ =>
+    unfold Frame.apply; simp; constructor
+    constructor; apply wf
+  case _ x =>
+    apply FrameWf.weaken (· + 1) _ _ (ih x)
+    constructor; apply wf
+    case _ =>
+      intro y; simp; unfold S; unfold Ren.to
+      simp
+case _ j1 j2 ih1 ih2 =>
+  intro x; cases x <;> simp at *
+  case _ =>
+    unfold Frame.apply; simp; constructor
+    have lem := weaken_type j1 j1; simp at lem
+    apply lem;
+  case _ x =>
+    apply FrameWf.weaken (· + 1) _ _ (ih2 x)
+    case _ => apply Judgment.wftype j1 j2
+    case _ =>
+      intro y; simp; unfold S; unfold Ren.to
+      simp
+case _ j1 j2 ih1 ih2 =>
+  intro x; cases x <;> simp at *
+  case _ =>
+    unfold Frame.apply; simp; constructor
+    have lem := weaken_kind j1 j1; simp at lem
+    apply lem;
+  case _ x =>
+    apply FrameWf.weaken (· + 1) _ _ (ih2 x)
+    case _ => apply Judgment.wfkind j1 j2
+    case _ =>
+      intro y; simp; unfold S; unfold Ren.to
+      simp
+case _ j1 j2 ih1 ih2 =>
+  intro x; cases x <;> simp at *
+  case _ =>
+    unfold Frame.apply; simp; constructor
+    have lem := weaken_datatype j1 j1; simp at lem
+    apply lem;
+  case _ x =>
+    apply FrameWf.weaken (· + 1) _ _ (ih2 x)
+    case _ => apply Judgment.wfdatatype j1 j2
+    case _ =>
+      intro y; simp; unfold S; unfold Ren.to
+      simp
+case _ j1 j2 j3 ih1 ih2 =>
+  intro x; cases x <;> simp at *
+  case _ =>
+    unfold Frame.apply; simp; constructor
+    have lem := weaken_ctor j1 j3 j1; simp at lem
+    apply lem; apply valid_ctor_subst _ _ j3
+    case _ =>
+      intro n y h; unfold S at h
+      injection h with e; subst e; simp
+    case _ =>
+      intro n h; exists n + 1
+  case _ x =>
+    apply FrameWf.weaken (· + 1) _ _ (ih2 x)
+    case _ => apply Judgment.wfctor j1 j2 j3
+    case _ =>
+      intro y; simp; unfold S; unfold Ren.to
+      simp
+case _ j1 j2 ih1 ih2 =>
+  intro x; cases x <;> simp at *
+  case _ =>
+    unfold Frame.apply; simp; constructor
+    have lem := weaken_opent j1 j1; simp at lem
+    apply lem;
+  case _ x =>
+    apply FrameWf.weaken (· + 1) _ _ (ih2 x)
+    case _ => apply Judgment.wfopent j1 j2
+    case _ =>
+      intro y; simp; unfold S; unfold Ren.to
+      simp
+case _ j1 j2 ih1 ih2 =>
+  intro x; cases x <;> simp at *
+  case _ =>
+    unfold Frame.apply; simp; constructor
+    have lem := weaken_openm j1 j1; simp at lem
+    apply lem;
+  case _ x =>
+    apply FrameWf.weaken (· + 1) _ _ (ih2 x)
+    case _ => apply Judgment.wfopenm j1 j2
+    case _ =>
+      intro y; simp; unfold S; unfold Ren.to
+      simp
+case _ j1 j2 j3 ih1 ih2 =>
+  intro x; cases x <;> simp at *
+  case _ =>
+    unfold Frame.apply; simp; constructor
+    have lem := weaken_insttype j1 j3 j1; simp at lem
+    apply lem; apply valid_insttype_subst _ _ j3
+    case _ =>
+      intro n y h; unfold S at h
+      injection h with e; subst e; simp
+    case _ =>
+      intro n h; exists n + 1
+  case _ x =>
+    apply FrameWf.weaken (· + 1) _ _ (ih2 x)
+    case _ => apply Judgment.wfinsttype j1 j2 j3
+    case _ =>
+      intro y; simp; unfold S; unfold Ren.to
+      simp
+case _ Γ x T t j1 j2 j3 ih1 ih2 =>
+  have lem1 : .openm ([S]T) = (Γ d@ x).apply S := by
+    rw [<-j1]; unfold Frame.apply; simp
+  intro x; cases x <;> simp at *
+  case _ =>
+    have lem2 := weaken_inst j1 j2 j2; simp at lem2
+    unfold Frame.apply; simp; constructor
+    simp; apply lem1; apply lem2
+  case _ x =>
+    apply FrameWf.weaken (· + 1) _ _ (ih2 x)
+    case _ => apply Judgment.wfinst j1 j2 j3
+    case _ =>
+      intro y; simp; unfold S; unfold Ren.to
+      simp
+case _ j1 j2 j3 ih1 ih2 ih3 =>
+  intro x; cases x <;> simp at *
+  case _ =>
+    have lem1 := weaken_term j1 j2 j1; simp at lem1
+    have lem2 := weaken_term j1 j2 j2; simp at lem2
+    unfold Frame.apply; simp; constructor
+    apply lem1; apply lem2
+  case _ x =>
+    apply FrameWf.weaken (· + 1) _ _ (ih3 x)
+    case _ => apply Judgment.wfterm j1 j2 j3
+    case _ =>
+      intro y; simp; unfold S; unfold Ren.to
+      simp
+
+theorem frame_wf_by_index x : ⊢ Γ -> Γ ⊢ Γ d@ x := by
+intro j;
+have lem := frame_wf_by_index_lemma j; simp at lem
+apply lem x
+
+theorem frame_wf_implies_typed_var T :
+  Γ ⊢ Γ d@ x ->
+  .some T = (Γ d@ x).get_type ->
+  Γ ⊢ #x : T
+:= by sorry
