SystemFD/Term.lean
@@ -2,4 +2,4 @@
 import SystemFD.Term.Definition
 import SystemFD.Term.Equality
 import SystemFD.Term.Substitution
-import SystemFD.Term.VariableSet
+import SystemFD.Term.Instances
