SystemFD/Term/Instances.lean
@@ -1,0 +1,178 @@
+import SystemFD.Substitution
+import SystemFD.Ctx
+import SystemFD.Term.Definition
+import SystemFD.Term.Substitution
+import SystemFD.Util
+
+@[simp]
+def instance_indices : Ctx Term -> Nat -> Nat -> List Nat -> List Nat
+| .nil , _,  _ , acc => acc
+| .cons (.inst (#x) _) Γ, n, opm , acc =>
+        (if opm == x + n + 1
+        then instance_indices Γ (n+1) opm (n::acc)
+        else instance_indices Γ (n+1) opm acc)
+| .cons _ Γ, n, opm , acc => instance_indices Γ (n + 1) opm acc
+
+theorem instance_indices_leq_implies_empty :
+  y ≤ x ->
+  instance_indices Γ x y ℓ = ℓ
+:= by
+intro h
+induction Γ, x, y, ℓ using instance_indices.induct
+case _ => simp
+case _ h2 ih =>
+  simp; split
+  case _ => exfalso; omega
+  case _ h3 =>
+    replace h2 := LawfulBEq.eq_of_beq h2
+    exfalso; omega
+case _ ih =>
+  simp; split
+  case _ => exfalso; omega
+  case _ => apply ih; omega
+case _ ih => simp; apply ih; omega
+
+theorem instance_indices_acc_append (Γ : Ctx Term) x y ℓ1 ℓ2 :
+  instance_indices Γ x y (ℓ1 ++ ℓ2) = instance_indices Γ x y ℓ1 ++ ℓ2
+:= by
+induction Γ, x, y, ℓ1 using instance_indices.induct generalizing ℓ2
+case _ => simp
+case _ h ih =>
+  simp at *; split
+  case _ => rw [ih]
+  case _ => exfalso; omega
+case _ ih =>
+  simp at *; split
+  case _ => exfalso; omega
+  case _ => rw [ih]
+case _ h ih => simp at *; rw [ih]
+
+theorem instance_indices_shift :
+  instance_indices Γ (x + k) (y + k) ℓ
+    = List.map (· + k) (instance_indices Γ x y []) ++ ℓ
+:= by
+generalize udef : x + k = u at *
+generalize vdef : y + k = v at *
+induction Γ, u, v, ℓ using instance_indices.induct generalizing x y k
+case _ => simp
+case _ z _ Γ n opm acc h ih =>
+  subst udef; subst vdef
+  simp at *; split
+  case _ =>
+    split
+    case _ acc e1 e2 =>
+      replace ih := @ih (x + 1) k y (by omega) (by omega)
+      have lem := instance_indices_acc_append Γ (x + 1) y [] [x]
+      simp at lem; rw [lem]; simp; rw [ih]
+    case _ => exfalso; omega
+  case _ => exfalso; omega
+case _ h ih =>
+  subst udef; subst vdef
+  simp at *; split
+  case _ => exfalso; omega
+  case _ z _ _ _ =>
+    cases y <;> simp at *
+    case _ =>
+      rw [instance_indices_leq_implies_empty]
+      rw [instance_indices_leq_implies_empty]
+      simp; omega; omega
+    case _ y _ =>
+      have ih := @ih (x + 1) k (y + 1) (by omega) (by omega)
+      split
+      case _ h => exfalso; omega
+      case _ => rw [<-ih]
+case _ h ih =>
+  subst udef; subst vdef
+  simp at *
+  replace ih := @ih (x + 1) k y (by omega) (by simp)
+  rw [ih]
+
+@[simp]
+def get_instances : Ctx Term -> List Nat -> List Term
+| _, [] => []
+| Γ, .cons i t =>
+  match Γ d@ i with
+  | .inst _ b => b :: get_instances Γ t
+  | _ => get_instances Γ t
+
+theorem instance_indices_sound : i ∈ instance_indices Γ k x [] -> ∃ t, (Γ d@ i) = .inst #x t := by
+intro j
+generalize ℓdef : [] = ℓ at *
+induction Γ, k, x, ℓ using instance_indices.induct generalizing i
+case _ => sorry
+case _ => sorry
+case _ => sorry
+case _ hd Γ n opm acc h ih =>
+  subst ℓdef; cases i <;> simp at *
+  case _ => sorry
+  case _ => sorry
+
+theorem get_instances_sound :
+  ix = instance_indices Γ k x [] ->
+  t ∈ get_instances Γ ix ->
+  ∃ i, Γ d@ i = .inst #x t
+:= by
+intro h1 h2
+induction Γ, ix using get_instances.induct generalizing x k t
+case _ => simp at *
+case _ Γ i ℓ a b h ih =>
+  simp at *; split at h2
+  case _ f u v e1 =>
+    simp at h2; cases h2
+    case _ h2 =>
+      subst h2; have lem : i ∈ instance_indices Γ k x [] := by sorry
+      replace lem := instance_indices_sound lem
+      cases lem; case _ t' lem =>
+        rw [e1] at lem; injection lem with e2 e3
+        subst e2; subst e3; exists i
+    case _ h2 =>
+      have lem : ∃ k', ℓ = instance_indices Γ k' x [] := by sorry
+      cases lem; case _ k' lem =>
+        replace ih := ih lem h2
+        apply ih
+  case _ =>
+    have lem : ∃ k', ℓ = instance_indices Γ k' x [] := by sorry
+    cases lem; case _ k' lem =>
+      replace ih := ih lem h2
+      apply ih
+case _ Γ i ℓ h ih =>
+  simp at *
+  have lem : ∃ k', ℓ = instance_indices Γ k' x [] := by sorry
+  cases lem; case _ k' lem =>
+    replace ih := ih lem h2
+    apply ih
+
+-- theorem get_instances_strengthen (f : Frame Term) :
+--   (∀ i n, .some n = ix.get? i -> n > 0) ->
+--   get_instances (f :: Γ) ix
+--     = List.map ([S]·) (get_instances Γ (List.map (· - 1) ix))
+-- := by
+-- intro h; induction ix generalizing f Γ
+-- case _ => simp
+-- case _ hd tl ih =>
+--   cases hd <;> simp at *
+--   case _ =>
+--     replace h := h 0 0 (by simp)
+--     exfalso; omega
+--   case _ x =>
+--     generalize zdef : Γ d@ x = z at *
+--     cases z
+--     case inst => sorry
+--     all_goals (
+--       unfold Frame.apply; simp at *
+--       rw [ih]
+--       intro i n h'
+--       replace h := h (i + 1) n; simp at h
+--       apply h h'
+--     )
+
+-- theorem get_instances_succ {f : Frame Term} :
+--   get_instances (f :: Γ) (instance_indices Γ (y + 1) (x + 1) [])
+--     = List.map ([S]·) (get_instances Γ (instance_indices Γ y x []))
+-- := by
+-- rw [instance_indices_shift]
+-- rw [get_instances_strengthen]; simp
+-- unfold Function.comp; simp
+-- intro i n h; simp at h
+-- generalize zdef : (instance_indices Γ y x [])[i]? = z at *
+-- cases z <;> simp at *; omega
